src/Testprog.v
@@ -12,7 +12,7 @@ Set Implicit Arguments.
 
 
 Definition copy_block T xp (a b : addr) mscs rx : prog T :=
-  let2 (mscs, v) <- MEMLOG.read xp a mscs;
+  let^ (mscs, v) <- MEMLOG.read xp a mscs;
   mscs <- MEMLOG.write xp b v mscs;
   rx mscs.
 
@@ -30,62 +30,63 @@ Definition testcopy T xp rx : prog T :=
   mscs <- MEMLOG.init xp cs ;
   mscs <- MEMLOG.begin xp mscs ;
   mscs <- copy_many xp 200 $100 $500 mscs ;
-  let2 (mscs, ok) <- MEMLOG.commit xp mscs ;
+  let^ (mscs, ok) <- MEMLOG.commit xp mscs ;
   rx ok.
 
 Definition testalloc T lxp bxp rx : prog T :=
   cs <- BUFCACHE.init 1000 ;
   mscs <- MEMLOG.init lxp cs ;
   mscs <- MEMLOG.begin lxp mscs ;
-  let2 (mscs, b) <- BALLOC.alloc lxp bxp mscs ;
+  let^ (mscs, b) <- BALLOC.alloc lxp bxp mscs ;
   match b with
   | None =>
     mscs <- MEMLOG.abort lxp mscs ;
     rx None
   | Some bn =>
     mscs <- MEMLOG.write lxp $0 (addr2valu bn) mscs ;
-    let2 (mscs, ok) <- MEMLOG.commit lxp mscs ;
+    let^ (mscs, ok) <- MEMLOG.commit lxp mscs ;
     rx (Some bn)
   end.
 
 Definition test_bfile T fsxp v mscs rx : prog T :=
   mscs <- MEMLOG.begin (FSXPMemLog fsxp) mscs ;
-  let2 (mscs, ok) <- BFILE.bfgrow (FSXPMemLog fsxp) (FSXPBlockAlloc fsxp) (FSXPInode fsxp) $3 mscs ;
+  let^ (mscs, ok) <- BFILE.bfgrow (FSXPMemLog fsxp) (FSXPBlockAlloc fsxp) (FSXPInode fsxp) $3 mscs ;
   match ok with
   | false =>
     mscs <- MEMLOG.abort (FSXPMemLog fsxp) mscs ;
-    rx (mscs, None)
+    rx ^(mscs, None)
   | true =>
     mscs <- BFILE.bfwrite (FSXPMemLog fsxp) (FSXPInode fsxp) $3 $0 v mscs ;
-    let2 (mscs, ok) <- MEMLOG.commit (FSXPMemLog fsxp) mscs ;
+    let^ (mscs, ok) <- MEMLOG.commit (FSXPMemLog fsxp) mscs ;
 
     match ok with
-    | false => rx (mscs, None)
+    | false => rx ^(mscs, None)
     | true =>
       mscs <- MEMLOG.begin (FSXPMemLog fsxp) mscs ;
-      let2 (mscs, b) <- BFILE.bfread (FSXPMemLog fsxp) (FSXPInode fsxp) $3 $0 mscs ;
+      let^ (mscs, b) <- BFILE.bfread (FSXPMemLog fsxp) (FSXPInode fsxp) $3 $0 mscs ;
       mscs <- BFILE.bfshrink (FSXPMemLog fsxp) (FSXPBlockAlloc fsxp) (FSXPInode fsxp) $3 mscs ;
-      let2 (mscs, ok) <- MEMLOG.commit (FSXPMemLog fsxp) mscs ;
+      let^ (mscs, ok) <- MEMLOG.commit (FSXPMemLog fsxp) mscs ;
       match ok with
-      | false => rx (mscs, None)
-      | true => rx (mscs, Some b)
+      | false => rx ^(mscs, None)
+      | true => rx ^(mscs, Some b)
       end
     end
   end.
 
 Definition test_bfile_bulkwrite T fsxp v nblocks mscs rx : prog T :=
   mscs <- MEMLOG.begin (FSXPMemLog fsxp) mscs;
-  mscs <- For block < nblocks
-    Loopvar mscs <- mscs
+  let^ (mscs) <- For block < nblocks
+    Ghost [ (_:unit) ]
+    Loopvar [ mscs ]
     Continuation lrx
     Invariant emp
     OnCrash emp
     Begin
       mscs <- BFILE.bfwrite (FSXPMemLog fsxp) (FSXPInode fsxp) $3 block v mscs;
-      lrx mscs
-  Rof;
-  let2 (mscs, ok) <- MEMLOG.commit (FSXPMemLog fsxp) mscs;
-  rx (mscs, ok).
+      lrx ^(mscs)
+  Rof ^(mscs);
+  let^ (mscs, ok) <- MEMLOG.commit (FSXPMemLog fsxp) mscs;
+  rx ^(mscs, ok).
 
 (* Why does this seemingly simple function take forever to compile?? *)
 (*
